Update bug with autominimization

safechecker/theories/PCUICSafeConversion.v
@@ -1,223 +1,9 @@
 (* -*- mode: coq; coq-prog-args: ("-emacs" "-q" "-w" "-deprecated-native-compiler-option" "-native-compiler" "no" "-R" "/github/workspace/metacoq/utils/theories" "MetaCoq.Utils" "-R" "/github/workspace/metacoq/common/theories" "MetaCoq.Common" "-R" "/github/workspace/metacoq/pcuic/theories" "MetaCoq.PCUIC" "-R" "/github/workspace/metacoq/safechecker/theories" "MetaCoq.SafeChecker" "-Q" "/github/workspace/cwd" "Top" "-Q" "/home/coq/.opam/4.13.1+flambda/lib/coq/user-contrib/Bignums" "Bignums" "-Q" "/home/coq/.opam/4.13.1+flambda/lib/coq/user-contrib/Equations" "Equations" "-Q" "/home/coq/.opam/4.13.1+flambda/lib/coq/user-contrib/Ltac2" "Ltac2" "-top" "MetaCoq.SafeChecker.PCUICSafeConversion") -*- *)
-(* File reduced by coq-bug-minimizer from original input, then from 5927 lines to 1512 lines *)
+(* File reduced by coq-bug-minimizer from original input, then from 5927 lines to 1512 lines, then from 1095 lines to 222 lines, then from 235 lines to 2362 lines, then from 2362 lines to 1248 lines *)
 (* coqc version 8.16.1 compiled with OCaml 4.13.1
    coqtop version 8.16.1
-   Expected coqc runtime on this file: 50.537 sec *)
+   Expected coqc runtime on this file: 112.421 sec *)
 Require Coq.Init.Ltac.
-Require Coq.Logic.ProofIrrelevance.
-Require Coq.Bool.Bool.
-Require Coq.ZArith.ZArith.
-Require Coq.Arith.Arith.
-Require Coq.micromega.Lia.
-Require Coq.Lists.List.
-Require Coq.Init.Nat.
-Require Coq.Strings.Ascii.
-Require Coq.Strings.String.
-Require Coq.Classes.Morphisms.
-Require Coq.extraction.Extraction.
-Require Coq.Unicode.Utf8_core.
-Require Equations.Init.
-Require Equations.Signature.
-Require Equations.CoreTactics.
-Require Coq.Relations.Relation_Definitions.
-Require Equations.Prop.Logic.
-Require Equations.Prop.Classes.
-Require Coq.Program.Tactics.
-Require Equations.Prop.EqDec.
-Require Equations.Prop.DepElim.
-Require Coq.Relations.Relations.
-Require Equations.Prop.Constants.
-Require Coq.Bool.Bvector.
-Require Coq.Arith.Wf_nat.
-Require Coq.Wellfounded.Wellfounded.
-Require Coq.Relations.Relation_Operators.
-Require Coq.Wellfounded.Lexicographic_Product.
-Require Coq.Program.Wf.
-Require Coq.Logic.FunctionalExtensionality.
-Require Equations.Prop.Subterm.
-Require Equations.Prop.FunctionalInduction.
-Require Equations.Prop.Tactics.
-Require Equations.Prop.NoConfusion.
-Require Equations.Prop.EqDecInstances.
-Require Equations.Prop.Loader.
-Require Equations.Prop.Telescopes.
-Require Equations.Prop.Equations.
-Require MetaCoq.Utils.MCPrelude.
-Require Coq.ssr.ssreflect.
-Require MetaCoq.Utils.MCReflect.
-Require Coq.Unicode.Utf8.
-Require Coq.Lists.SetoidList.
-Require Coq.Classes.CRelationClasses.
-Require Equations.Type.Logic.
-Require Equations.Type.Relation.
-Require Equations.Type.Relation_Properties.
-Require MetaCoq.Utils.MCRelations.
-Require Coq.ssr.ssrbool.
-Require MetaCoq.Utils.ReflectEq.
-Require MetaCoq.Utils.MCList.
-Require Coq.Classes.RelationClasses.
-Require MetaCoq.Utils.MCProd.
-Require MetaCoq.Utils.MCOption.
-Require MetaCoq.Utils.MCSquash.
-Require MetaCoq.Utils.All_Forall.
-Require MetaCoq.Utils.MCArith.
-Require Coq.Structures.OrderedType.
-Require Coq.Structures.Orders.
-Require MetaCoq.Utils.MCCompare.
-Require MetaCoq.Utils.MCEquality.
-Require Coq.Init.Decimal.
-Require Coq.Numbers.DecimalString.
-Require Coq.NArith.NArith.
-Require Coq.Strings.Byte.
-Require Coq.NArith.BinNat.
-Require MetaCoq.Utils.ByteCompare.
-Require MetaCoq.Utils.ByteCompareSpec.
-Require MetaCoq.Utils.bytestring.
-Require MetaCoq.Utils.MCString.
-Require MetaCoq.Utils.MCTactics.SpecializeBy.
-Require MetaCoq.Utils.MCTactics.Zeta1.
-Require MetaCoq.Utils.MCTactics.GeneralizeOverHoles.
-Require MetaCoq.Utils.MCTactics.FindHyp.
-Require MetaCoq.Utils.MCTactics.UniquePose.
-Require MetaCoq.Utils.MCTactics.InHypUnderBindersDo.
-Require MetaCoq.Utils.MCTactics.SpecializeUnderBindersBy.
-Require MetaCoq.Utils.MCTactics.Head.
-Require MetaCoq.Utils.MCTactics.DestructHyps.
-Require MetaCoq.Utils.MCTactics.DestructHead.
-Require MetaCoq.Utils.MCTactics.SpecializeAllWays.
-Require MetaCoq.Utils.MCTactics.SplitInContext.
-Require Ltac2.Init.
-Require Ltac2.Message.
-Require Ltac2.Control.
-Require Ltac2.Ltac1.
-Require MetaCoq.Utils.MCUtils.
-Require MetaCoq.Utils.monad_utils.
-Require MetaCoq.Utils.utils.
-Require Coq.btauto.Btauto.
-Require MetaCoq.Common.config.
-Require Coq.Structures.OrderedTypeAlt.
-Require Coq.MSets.MSetAVL.
-Require Coq.MSets.MSetFacts.
-Require Coq.MSets.MSetProperties.
-Require Coq.MSets.MSetDecide.
-Require Coq.ZArith.Zcompare.
-Require Coq.MSets.MSetInterface.
-Require MetaCoq.Utils.wGraph.
-Require Coq.Structures.OrdersAlt.
-Require Coq.MSets.MSetList.
-Require Coq.FSets.FMapAVL.
-Require Coq.Setoids.Setoid.
-Require Coq.Structures.OrderedTypeEx.
-Require Coq.FSets.FMapFacts.
-Require MetaCoq.Common.Kernames.
-Require Coq.Floats.SpecFloat.
-Require MetaCoq.Common.BasicAst.
-Require MetaCoq.Common.Universes.
-Require Coq.Classes.SetoidTactics.
-Require MetaCoq.Common.uGraph.
-Require Coq.ssr.ssrfun.
-Require Coq.Numbers.Cyclic.Int63.Uint63.
-Require Coq.Floats.PrimFloat.
-Require Coq.Floats.FloatOps.
-Require Coq.Numbers.HexadecimalString.
-Require MetaCoq.Common.Primitive.
-Require MetaCoq.Common.Environment.
-Require Coq.Floats.FloatAxioms.
-Require MetaCoq.Common.Reflect.
-Require Coq.Classes.CMorphisms.
-Require MetaCoq.Common.EnvironmentTyping.
-Require MetaCoq.PCUIC.utils.PCUICPrimitive.
-Require MetaCoq.PCUIC.PCUICAst.
-Require MetaCoq.PCUIC.utils.PCUICSize.
-Require MetaCoq.PCUIC.utils.PCUICAstUtils.
-Require Coq.Program.Program.
-Require Coq.PArith.BinPos.
-Require Coq.Arith.Compare_dec.
-Require MetaCoq.Utils.LibHypsNaming.
-Require MetaCoq.PCUIC.Syntax.PCUICCases.
-Require MetaCoq.PCUIC.Syntax.PCUICInduction.
-Require MetaCoq.PCUIC.Syntax.PCUICReflect.
-Require MetaCoq.PCUIC.Syntax.PCUICLiftSubst.
-Require MetaCoq.PCUIC.Syntax.PCUICUnivSubst.
-Require MetaCoq.PCUIC.PCUICEquality.
-Require MetaCoq.PCUIC.utils.PCUICUtils.
-Require MetaCoq.PCUIC.Syntax.PCUICPosition.
-Require MetaCoq.PCUIC.utils.PCUICOnOne.
-Require MetaCoq.Utils.MCPred.
-Require MetaCoq.PCUIC.PCUICSigmaCalculus.
-Require MetaCoq.PCUIC.Syntax.PCUICClosed.
-Require MetaCoq.PCUIC.Syntax.PCUICOnFreeVars.
-Require MetaCoq.PCUIC.PCUICCumulativitySpec.
-Require MetaCoq.PCUIC.PCUICTyping.
-Require MetaCoq.PCUIC.PCUICGlobalEnv.
-Require MetaCoq.PCUIC.Syntax.PCUICTactics.
-Require MetaCoq.PCUIC.PCUICReduction.
-Require MetaCoq.PCUIC.PCUICCumulativity.
-Require MetaCoq.PCUIC.PCUICContextSubst.
-Require MetaCoq.PCUIC.PCUICWeakeningEnv.
-Require MetaCoq.PCUIC.Conversion.PCUICWeakeningEnvConv.
-Require MetaCoq.PCUIC.Syntax.PCUICNamelessDef.
-Require MetaCoq.PCUIC.Syntax.PCUICRenameDef.
-Require MetaCoq.PCUIC.Syntax.PCUICInstDef.
-Require MetaCoq.PCUIC.PCUICGuardCondition.
-Require MetaCoq.PCUIC.Typing.PCUICWeakeningEnvTyp.
-Require MetaCoq.PCUIC.Conversion.PCUICClosedConv.
-Require MetaCoq.PCUIC.Typing.PCUICClosedTyp.
-Require MetaCoq.PCUIC.Syntax.PCUICViews.
-Require MetaCoq.PCUIC.Conversion.PCUICRenameConv.
-Require MetaCoq.PCUIC.Conversion.PCUICWeakeningConv.
-Require MetaCoq.PCUIC.Conversion.PCUICOnFreeVarsConv.
-Require MetaCoq.PCUIC.Typing.PCUICRenameTyp.
-Require MetaCoq.PCUIC.Typing.PCUICWeakeningTyp.
-Require MetaCoq.PCUIC.Conversion.PCUICUnivSubstitutionConv.
-Require MetaCoq.PCUIC.Conversion.PCUICInstConv.
-Require MetaCoq.PCUIC.Typing.PCUICInstTyp.
-Require MetaCoq.PCUIC.PCUICSubstitution.
-Require MetaCoq.PCUIC.PCUICContextReduction.
-Require MetaCoq.PCUIC.Syntax.PCUICDepth.
-Require MetaCoq.PCUIC.PCUICParallelReduction.
-Require MetaCoq.PCUIC.PCUICParallelReductionConfluence.
-Require MetaCoq.PCUIC.PCUICRedTypeIrrelevance.
-Require MetaCoq.PCUIC.PCUICConfluence.
-Require MetaCoq.PCUIC.PCUICWellScopedCumulativity.
-Require MetaCoq.PCUIC.PCUICContextConversion.
-Require MetaCoq.PCUIC.PCUICConversion.
-Require MetaCoq.PCUIC.PCUICCasesContexts.
-Require MetaCoq.PCUIC.PCUICGeneration.
-Require MetaCoq.PCUIC.Typing.PCUICContextConversionTyp.
-Require MetaCoq.PCUIC.PCUICInversion.
-Require MetaCoq.PCUIC.Typing.PCUICUnivSubstitutionTyp.
-Require MetaCoq.PCUIC.PCUICContexts.
-Require MetaCoq.PCUIC.PCUICWfUniverses.
-Require MetaCoq.PCUIC.PCUICArities.
-Require MetaCoq.PCUIC.PCUICSpine.
-Require MetaCoq.PCUIC.PCUICInductives.
-Require MetaCoq.PCUIC.PCUICValidity.
-Require MetaCoq.PCUIC.PCUICInductiveInversion.
-Require MetaCoq.PCUIC.PCUICAlpha.
-Require MetaCoq.PCUIC.PCUICSR.
-Require MetaCoq.PCUIC.PCUICNormal.
-Require MetaCoq.PCUIC.PCUICSafeLemmata.
-Require MetaCoq.PCUIC.PCUICCumulProp.
-Require MetaCoq.PCUIC.PCUICPrincipality.
-Require MetaCoq.PCUIC.PCUICSN.
-Require MetaCoq.PCUIC.PCUICConvCumInversion.
-Require MetaCoq.PCUIC.utils.PCUICPretty.
-Require MetaCoq.SafeChecker.PCUICErrors.
-Require MetaCoq.Utils.canonicaltries.String2pos.
-Require MetaCoq.Utils.canonicaltries.CanonicalTries.
-Require MetaCoq.Common.EnvMap.
-Require MetaCoq.SafeChecker.PCUICEqualityDec.
-Require MetaCoq.SafeChecker.PCUICWfEnv.
-Require MetaCoq.PCUIC.PCUICCSubst.
-Require MetaCoq.PCUIC.PCUICWcbvEval.
-Require MetaCoq.PCUIC.PCUICElimination.
-Require MetaCoq.PCUIC.PCUICCanonicity.
-Require Equations.Type.FunctionalExtensionality.
-Require Equations.Type.WellFounded.
-Require MetaCoq.SafeChecker.PCUICWfReduction.
-Require MetaCoq.SafeChecker.PCUICSafeReduce.
-
 Module Export AdmitTactic.
 Module Import LocalFalse.
 Inductive False : Prop := .
@@ -226,48 +12,176 @@ Axiom proof_admitted : False.
 Import Coq.Init.Ltac.
 Tactic Notation "admit" := abstract case proof_admitted.
 End AdmitTactic.
-Import Coq.Logic.ProofIrrelevance.
-Import MetaCoq.Utils.utils.
-Import MetaCoq.Common.config MetaCoq.Common.uGraph.
-Import MetaCoq.PCUIC.PCUICAst MetaCoq.PCUIC.utils.PCUICAstUtils
-     MetaCoq.PCUIC.Syntax.PCUICReflect MetaCoq.PCUIC.Syntax.PCUICLiftSubst MetaCoq.PCUIC.Syntax.PCUICUnivSubst MetaCoq.PCUIC.PCUICTyping MetaCoq.PCUIC.PCUICGlobalEnv
-     MetaCoq.PCUIC.PCUICCumulativity MetaCoq.PCUIC.PCUICConversion MetaCoq.PCUIC.PCUICEquality MetaCoq.PCUIC.PCUICConversion
-     MetaCoq.PCUIC.PCUICSafeLemmata MetaCoq.PCUIC.PCUICNormal MetaCoq.PCUIC.PCUICInversion MetaCoq.PCUIC.PCUICReduction MetaCoq.PCUIC.Syntax.PCUICPosition
-     MetaCoq.PCUIC.PCUICPrincipality MetaCoq.PCUIC.PCUICContextConversion MetaCoq.PCUIC.Typing.PCUICContextConversionTyp MetaCoq.PCUIC.PCUICSN MetaCoq.PCUIC.utils.PCUICUtils MetaCoq.PCUIC.PCUICWfUniverses
-     MetaCoq.PCUIC.Syntax.PCUICOnFreeVars MetaCoq.PCUIC.PCUICWellScopedCumulativity
-     MetaCoq.PCUIC.Conversion.PCUICWeakeningEnvConv MetaCoq.PCUIC.Typing.PCUICWeakeningEnvTyp
-     MetaCoq.PCUIC.Conversion.PCUICWeakeningConv MetaCoq.PCUIC.Typing.PCUICWeakeningTyp
-     MetaCoq.PCUIC.Syntax.PCUICClosed MetaCoq.PCUIC.Typing.PCUICClosedTyp MetaCoq.PCUIC.PCUICConvCumInversion .
-Import MetaCoq.SafeChecker.PCUICErrors MetaCoq.SafeChecker.PCUICWfEnv MetaCoq.SafeChecker.PCUICSafeReduce MetaCoq.SafeChecker.PCUICEqualityDec.
-Import Equations.Prop.DepElim.
-Import Equations.Prop.Equations.
+Module MetaCoq_DOT_SafeChecker_DOT_PCUICSafeReduce_WRAPPED.
+Module PCUICSafeReduce.
+ 
 
-Local Set Keyed Unification.
+Require Coq.Classes.RelationClasses.
+Import Coq.Classes.RelationClasses.
+
+Require MetaCoq.Utils.utils.
+Import MetaCoq.Utils.utils.
+
+Require MetaCoq.Common.config.
+Import MetaCoq.Common.config.
+
+Require MetaCoq.PCUIC.PCUICCanonicity.
+Require MetaCoq.PCUIC.PCUICWellScopedCumulativity.
+Require MetaCoq.PCUIC.Syntax.PCUICOnFreeVars.
+Require MetaCoq.PCUIC.PCUICConversion.
+Require MetaCoq.PCUIC.PCUICConfluence.
+Require MetaCoq.PCUIC.PCUICSafeLemmata.
+Require MetaCoq.PCUIC.PCUICValidity.
+Require MetaCoq.PCUIC.PCUICReduction.
+Require MetaCoq.PCUIC.utils.PCUICUtils.
+Require MetaCoq.PCUIC.PCUICSN.
+Require MetaCoq.PCUIC.PCUICSR.
+Require MetaCoq.PCUIC.PCUICInversion.
+Require MetaCoq.PCUIC.PCUICNormal.
+Require MetaCoq.PCUIC.Syntax.PCUICPosition.
+Require MetaCoq.PCUIC.PCUICTyping.
+Require MetaCoq.PCUIC.Syntax.PCUICUnivSubst.
+Require MetaCoq.PCUIC.Syntax.PCUICLiftSubst.
+Require MetaCoq.PCUIC.PCUICGeneration.
+Require MetaCoq.PCUIC.utils.PCUICAstUtils.
+Require MetaCoq.PCUIC.PCUICAst.
+Import MetaCoq.PCUIC.PCUICAst MetaCoq.PCUIC.utils.PCUICAstUtils
+     MetaCoq.PCUIC.PCUICGeneration MetaCoq.PCUIC.Syntax.PCUICLiftSubst
+     MetaCoq.PCUIC.Syntax.PCUICUnivSubst MetaCoq.PCUIC.PCUICTyping MetaCoq.PCUIC.Syntax.PCUICPosition MetaCoq.PCUIC.PCUICNormal
+     MetaCoq.PCUIC.PCUICInversion MetaCoq.PCUIC.PCUICSR MetaCoq.PCUIC.PCUICSN
+     MetaCoq.PCUIC.utils.PCUICUtils MetaCoq.PCUIC.PCUICReduction MetaCoq.PCUIC.PCUICValidity MetaCoq.PCUIC.PCUICSafeLemmata
+     MetaCoq.PCUIC.PCUICConfluence MetaCoq.PCUIC.PCUICConversion
+     MetaCoq.PCUIC.Syntax.PCUICOnFreeVars MetaCoq.PCUIC.PCUICWellScopedCumulativity
+     MetaCoq.PCUIC.PCUICCanonicity.
+
+
+Require MetaCoq.SafeChecker.PCUICWfEnv.
+Require MetaCoq.SafeChecker.PCUICWfReduction.
+Require MetaCoq.SafeChecker.PCUICErrors.
+Import MetaCoq.SafeChecker.PCUICErrors MetaCoq.SafeChecker.PCUICWfReduction MetaCoq.SafeChecker.PCUICWfEnv.
+
+
+Require Equations.Prop.DepElim.
+Import Equations.Prop.DepElim.
+
+Require Equations.Prop.Equations.
+Import Equations.Prop.Equations.
+Set Equations Transparent.
+Set Equations With UIP.
+
+ 
+
+ 
+Notation " `  t " := (proj1_sig t) (at level 10, t at next level) : metacoq_scope.
 
 Set Default Goal Selector "!".
 
+Local Set Keyed Unification.
+
 Implicit Types (cf : checker_flags) (Σ : global_env_ext).
 
-#[global]
-Instance red_brs_refl Σ p Γ: CRelationClasses.Reflexive (@red_brs Σ p Γ).
+Lemma welltyped_is_closed_context {cf Σ} {wfΣ : wf Σ} {Γ t} :
+  welltyped Σ Γ t -> is_closed_context Γ.
+Admitted.
+#[global] Hint Resolve welltyped_is_closed_context : fvs.
+
+Lemma welltyped_is_open_term {cf Σ} {wfΣ : wf Σ} {Γ t} :
+  welltyped Σ Γ t -> is_open_term Γ t.
+Admitted.
+#[global] Hint Resolve welltyped_is_open_term : fvs.
+
+ 
+Section Measure.
+
+  Context {cf : checker_flags} {no : normalizing_flags}.
+
+  Context (flags : RedFlags.t).
+  Context (Σ : global_env_ext).
+
+  Definition R_aux Γ :=
+    dlexprod (cored Σ Γ) (@posR).
+
+  Definition R Γ u v :=
+    R_aux Γ (zip u ; stack_pos (fst u) (snd u))
+            (zip v ; stack_pos (fst v) (snd v)).
+
+  Lemma cored_welltyped :
+    forall {Γ u v},
+      wf Σ -> welltyped Σ Γ u ->
+      cored Σ Γ v u ->
+      welltyped Σ Γ v.
 Admitted.
 
-#[global]
-Instance conv_cum_trans {cf leq} {Σ : global_env_ext} {Γ} : wf Σ -> RelationClasses.Transitive (@conv_cum cf leq Σ Γ).
+  Lemma red_welltyped :
+    forall {Γ u v},
+      wf Σ -> welltyped Σ Γ u ->
+      red (fst Σ) Γ u v ->
+      welltyped Σ Γ v.
 Admitted.
 
-Lemma closed_red_mkApps_tConst_axiom {cf} {Σ} {wfΣ : wf Σ} {Γ} {cst u} {args : list term} {cb c} :
-  declared_constant Σ cst cb -> cst_body cb = None ->
-  Σ ;;; Γ ⊢ mkApps (tConst cst u) args ⇝ c ->
-  ∑ args' : list term,
-  (c = mkApps (tConst cst u) args') * (red_terms Σ Γ args args').
+  Derive Signature for Acc.
+  Lemma R_positionR :
+    forall Γ t1 t2 (p1 : pos t1) (p2 : pos t2),
+      t1 = t2 ->
+      positionR (` p1) (` p2) ->
+      R_aux Γ (t1 ; p1) (t2 ; p2).
 Admitted.
 
+  Definition Req Γ t t' :=
+    t = t' \/ R Γ t t'.
 
+  Lemma Rtrans :
+    forall Γ u v w,
+      R Γ u v ->
+      R Γ v w ->
+      R Γ u w.
+admit.
+Defined.
 
-Section Conversion.
+  Lemma Req_trans :
+    forall {Γ}, Transitive (Req Γ).
+admit.
+Defined.
 
-  Context {cf : checker_flags} {nor : normalizing_flags}.
+  Lemma R_to_Req :
+    forall {Γ u v},
+      R Γ u v ->
+      Req Γ u v.
+admit.
+Defined.
+
+  Instance Req_refl : forall Γ, Reflexive (Req Γ).
+Admitted.
+
+  Lemma R_Req_R :
+    forall {Γ u v w},
+      R Γ u v ->
+      Req Γ v w ->
+      R Γ u w.
+Admitted.
+
+End Measure.
+
+ 
+Section Acc_sidecond_generator.
+  Context {A : Type} {R : A -> A -> Prop} {P : A -> Prop}.
+  Variable Pimpl : forall x y, P x -> R y x -> P y.
+   
+  Fixpoint Acc_intro_generator n (acc : forall t, P t -> Acc R t) : forall t, P t -> Acc R t :=
+    match n with
+        | O => acc
+        | S n => fun x Px =>
+                   Acc_intro x (fun y Hy => Acc_intro_generator n (Acc_intro_generator n acc) y (Pimpl _ _ Px Hy))
+    end.
+End Acc_sidecond_generator.
+ 
+Opaque Acc_intro_generator.
+
+Section Reduce.
+
+  Context {cf : checker_flags} {no : normalizing_flags}.
+
+  Context (flags : RedFlags.t).
 
   Context (X_type : abstract_env_impl).
 
@@ -275,14 +189,869 @@ Section Conversion.
 
   Context {normalization_in : forall Σ, wf_ext Σ -> Σ ∼_ext X -> NormalizationIn Σ}.
 
+ 
+
   Local Definition heΣ Σ (wfΣ : abstract_env_ext_rel X Σ) :
     ∥ wf_ext Σ ∥ :=  abstract_env_ext_wf _ wfΣ.
 
   Local Definition hΣ Σ (wfΣ : abstract_env_ext_rel X Σ) :
     ∥ wf Σ ∥ := abstract_env_ext_sq_wf _ _ _ wfΣ.
 
-  Set Equations Transparent.
-  Set Equations With UIP.
+  Existing Instance Req_refl.
+
+Lemma acc_dlexprod_gen P Q A B (leA : P -> A -> A -> Prop)
+  (HQ : ∥ ∑ p , Q p ∥)
+  (HP : forall p p' x x', Q p -> Q p' -> leA p x x' -> leA p' x x')
+  (leB : forall x : A, B x -> B x -> Prop) :
+  (forall x, well_founded (leB x)) ->
+  forall x,
+    Acc (fun t t' => forall (p:P), Q p -> leA p t t') x ->
+    forall y,
+      Acc (leB x) y ->
+      Acc (fun t t' => forall (p:P), Q p -> @dlexprod A B (leA p) leB t t') (x;y).
+admit.
+Defined.
+
+Lemma dlexprod_Acc_gen P Q A B (leA : P -> A -> A -> Prop)
+  (HQ : ∥ ∑ p , Q p ∥)
+  (HP : forall p p' x x', Q p -> Q p' -> leA p x x' -> leA p' x x')
+  (leB : forall x : A, B x -> B x -> Prop) :
+    (forall x, well_founded (leB x)) ->
+    forall x y,
+      Acc (fun t t' => forall (p:P), Q p -> leA p t t') x ->
+      Acc (fun t t' => forall (p:P), Q p -> @dlexprod A B (leA p) leB t t') (x;y).
+admit.
+Defined.
+
+Definition R_singleton Abs A
+  (R : Abs -> A -> A -> Prop) (Q : Abs -> Prop) x (q : Q x)
+  (HQ : forall x x' , Q x -> Q x' -> x = x') (a a' : A) :
+  R x a a' <-> (forall x, Q x -> R x a a').
+Proof using Type.
+  split.
+  -
+ intros H x' q'.
+ specialize (HQ x x' q q').
+subst; eauto.
+  -
+ eauto.
+Defined.
+
+Fixpoint Acc_equiv A (R R' : A -> A -> Prop)
+  (Heq : forall a a', R a a' <-> R' a a') a
+  (HAcc : Acc R a) : Acc R' a.
+Proof using Type.
+  econstructor.
+intros.
+apply Heq in H.
+  destruct HAcc.
+eapply Acc_equiv; eauto.
+Defined.
+
+Corollary R_Acc_aux :
+    forall Γ t p,
+    (forall Σ (wfΣ : abstract_env_ext_rel X Σ), welltyped Σ Γ t) ->
+    (Acc (fun t t' => forall Σ (wfΣ : abstract_env_ext_rel X Σ), R_aux Σ Γ t t') (t ; p)).
+  Proof using normalization_in.
+    intros Γ t p h.
+    eapply dlexprod_Acc_gen.
+    -
+ apply abstract_env_ext_exists.
+    -
+ intros.
+eapply abstract_env_cored; try apply H1; eauto.
+    -
+ intros x.
+unfold well_founded.
+      eapply posR_Acc.
+    -
+ destruct (abstract_env_ext_exists X) as [[Σ wfΣ]];
+      destruct (heΣ _ wfΣ).
+      eapply Acc_equiv; try
+      eapply normalization_in; eauto.
+      eapply R_singleton with (Q := abstract_env_ext_rel X)
+          (R := fun Σ a a' => cored Σ Γ a a'); eauto.
+      intros; eapply abstract_env_ext_irr; eauto.
+  Defined.
+
+  Corollary R_Acc :
+    forall Γ t,
+      (forall Σ (wfΣ : abstract_env_ext_rel X Σ), welltyped Σ Γ (zip t)) ->
+      Acc (fun t t' => forall Σ (wfΣ : abstract_env_ext_rel X Σ), R Σ Γ t t') t.
+admit.
+Defined.
+
+  Definition inspect {A} (x : A) : { y : A | y = x } := exist x eq_refl.
+
+  Definition Pr (t' : term * stack) π :=
+    snd (decompose_stack π) = snd (decompose_stack (snd t')).
+
+  Notation givePr := (_) (only parsing).
+
+  Definition Pr' (t' : term * stack) :=
+    isApp (fst t') = false /\
+    (RedFlags.beta flags -> isLambda (fst t') -> isStackApp (snd t') = false).
+
+  Notation givePr' := (conj _ (fun β hl => _)) (only parsing).
+
+  Notation rec reduce t π :=
+    (let smaller := _ in
+     let '(exist res prf_Σ) := reduce t π smaller in
+     exist res (fun Σ wfΣ => let '((conj prf (conj h (conj h1 h2)))) := prf_Σ Σ wfΣ in conj (Req_trans _ _ _ _ _ (R_to_Req _ (smaller Σ wfΣ))) (conj givePr givePr'))
+    ) (only parsing).
+
+  Notation give t π :=
+    (exist (t,π) (fun Σ wfΣ => conj _ (conj givePr givePr'))) (only parsing).
+
+  Tactic Notation "zip" "fold" "in" hyp(h) :=
+    lazymatch type of h with
+    | context C[ zipc ?t ?π ] =>
+      let C' := context C[ zip (t,π) ] in
+      change C' in h
+    end.
+
+  Tactic Notation "zip" "fold" :=
+    lazymatch goal with
+    | |- context C[ zipc ?t ?π ] =>
+      let C' := context C[ zip (t,π) ] in
+      change C'
+    end.
+
+  Lemma Req_red Σ :
+    forall Γ x y,
+      Req Σ Γ y x ->
+      ∥ red Σ Γ (zip x) (zip y) ∥.
+admit.
+Defined.
+
+   
+  Ltac obTac :=
+     
+    Program.Tactics.program_simplify ;
+    Equations.CoreTactics.equations_simpl ;
+    try Program.Tactics.program_solve_wf ;
+    try reflexivity.
+
+  Obligation Tactic := obTac.
+
+  Equations discr_construct (t : term) : Prop :=
+    discr_construct (tConstruct ind n ui) := False ;
+    discr_construct _ := True.
+
+  Inductive construct_view : term -> Type :=
+  | view_construct : forall ind n ui, construct_view (tConstruct ind n ui)
+  | view_other : forall t, discr_construct t -> construct_view t.
+
+  Equations construct_viewc t : construct_view t :=
+    construct_viewc (tConstruct ind n ui) := view_construct ind n ui ;
+    construct_viewc t := view_other t I.
+
+   
+  Equations red_discr (t : term) (π : stack) : Prop :=
+    red_discr (tRel _) _ := False ;
+    red_discr (tLetIn _ _ _ _) _ := False ;
+    red_discr (tConst _ _) _ := False ;
+    red_discr (tApp _ _) _ := False ;
+    red_discr (tLambda _ _ _) (App_l _ :: _) := False ;
+    red_discr (tFix _ _) _ := False ;
+    red_discr (tCase _ _ _ _) _ := False ;
+    red_discr (tProj _ _) _ := False ;
+    red_discr _ _ := True.
+
+  Inductive red_view : term -> stack -> Type :=
+  | red_view_Rel c π : red_view (tRel c) π
+  | red_view_LetIn A b B c π : red_view (tLetIn A b B c) π
+  | red_view_Const c u π : red_view (tConst c u) π
+  | red_view_App f a π : red_view (tApp f a) π
+  | red_view_Lambda na A t a args : red_view (tLambda na A t) (App_l a :: args)
+  | red_view_Fix mfix idx π : red_view (tFix mfix idx) π
+  | red_view_Case ci p c brs π : red_view (tCase ci p c brs) π
+  | red_view_Proj p c π : red_view (tProj p c) π
+  | red_view_other t π : red_discr t π -> red_view t π.
+
+  Equations red_viewc t π : red_view t π :=
+    red_viewc (tRel c) π := red_view_Rel c π ;
+    red_viewc (tLetIn A b B c) π := red_view_LetIn A b B c π ;
+    red_viewc (tConst c u) π := red_view_Const c u π ;
+    red_viewc (tApp f a) π := red_view_App f a π ;
+    red_viewc (tLambda na A t) (App_l a :: args) := red_view_Lambda na A t a args ;
+    red_viewc (tFix mfix idx) π := red_view_Fix mfix idx π ;
+    red_viewc (tCase ci p c brs) π := red_view_Case ci p c brs π ;
+    red_viewc (tProj p c) π := red_view_Proj p c π ;
+    red_viewc t π := red_view_other t π I.
+
+  Equations discr_construct_cofix (t : term) : Prop :=
+    discr_construct_cofix (tConstruct ind n ui) := False ;
+    discr_construct_cofix (tCoFix mfix idx) := False ;
+    discr_construct_cofix _ := True.
+
+  Inductive construct_cofix_view : term -> Type :=
+  | ccview_construct : forall ind n ui, construct_cofix_view (tConstruct ind n ui)
+  | ccview_cofix : forall mfix idx, construct_cofix_view (tCoFix mfix idx)
+  | ccview_other : forall t, discr_construct_cofix t -> construct_cofix_view t.
+
+  Equations cc_viewc t : construct_cofix_view t :=
+    cc_viewc (tConstruct ind n ui) := ccview_construct ind n ui ;
+    cc_viewc (tCoFix mfix idx) := ccview_cofix mfix idx ;
+    cc_viewc t := ccview_other t I.
+
+  Equations discr_construct0_cofix (t : term) : Prop :=
+    discr_construct0_cofix (tConstruct ind n ui) := n <> 0 ;
+    discr_construct0_cofix (tCoFix mfix idx) := False ;
+    discr_construct0_cofix _ := True.
+
+  Inductive construct0_cofix_view : term -> Type :=
+  | cc0view_construct : forall ind ui, construct0_cofix_view (tConstruct ind 0 ui)
+  | cc0view_cofix : forall mfix idx, construct0_cofix_view (tCoFix mfix idx)
+  | cc0view_other : forall t, discr_construct0_cofix t -> construct0_cofix_view t.
+
+  Equations cc0_viewc t : construct0_cofix_view t :=
+    cc0_viewc (tConstruct ind 0 ui) := cc0view_construct ind ui ;
+    cc0_viewc (tCoFix mfix idx) := cc0view_cofix mfix idx ;
+    cc0_viewc t := cc0view_other t _.
+
+  Equations _reduce_stack (Γ : context) (t : term) (π : stack)
+            (h : forall Σ (wfΣ : abstract_env_ext_rel X Σ), welltyped Σ Γ (zip (t,π)))
+            (reduce : forall t' π', (forall Σ (wfΣ : abstract_env_ext_rel X Σ), R Σ Γ (t',π') (t,π)) ->
+                               { t'' : term * stack | forall Σ (wfΣ : abstract_env_ext_rel X Σ), Req Σ Γ t'' (t',π') /\ Pr t'' π' /\ Pr' t'' })
+    : { t' : term * stack | forall Σ (wfΣ : abstract_env_ext_rel X Σ), Req Σ Γ t' (t,π) /\ Pr t' π /\ Pr' t' } :=
+
+    _reduce_stack Γ t π h reduce with red_viewc t π := {
+
+    | red_view_Rel c π with RedFlags.zeta flags := {
+      | true with inspect (nth_error (Γ ,,, stack_context π) c) := {
+        | @exist None eq := False_rect _ _ ;
+        | @exist (Some d) eq with inspect d.(decl_body) := {
+          | @exist None _ := give (tRel c) π ;
+          | @exist (Some b) H := rec reduce (lift0 (S c) b) π
+          }
+        } ;
+      | false := give (tRel c) π
+      } ;
+
+    | red_view_LetIn A b B c π with RedFlags.zeta flags := {
+      | true := rec reduce (subst10 b c) π ;
+      | false := give (tLetIn A b B c) π
+      } ;
+
+    | red_view_Const c u π with RedFlags.delta flags := {
+      | true with inspect (abstract_env_lookup X c) := {
+        | @exist (Some (ConstantDecl {| cst_body := Some body |})) eq :=
+          let body' := subst_instance u body in
+          rec reduce body' π ;
+        | @exist (Some (InductiveDecl _)) eq := False_rect _ _ ;
+        | @exist (Some _) eq := give (tConst c u) π ;
+        | @exist None eq := False_rect _ _
+        } ;
+      | _ := give (tConst c u) π
+      } ;
+
+    | red_view_App f a π := rec reduce f (App_l a :: π) ;
+
+    | red_view_Lambda na A t a args with inspect (RedFlags.beta flags) := {
+      | @exist true eq1 := rec reduce (subst10 a t) args ;
+      | @exist false eq1 := give (tLambda na A t) (App_l a :: args)
+      } ;
+
+    | red_view_Fix mfix idx π with RedFlags.fix_ flags := {
+      | true with inspect (unfold_fix mfix idx) := {
+        | @exist (Some (narg, fn)) eq1 with inspect (decompose_stack_at π narg) := {
+          | @exist (Some (args, c, ρ)) eq2 with inspect (reduce c (Fix_app mfix idx args :: ρ) _) := {
+            | @exist (@exist (t, ρ') prf) eq3 with construct_viewc t := {
+              | view_construct ind n ui with inspect (decompose_stack ρ') := {
+                | @exist (l, θ) eq4 :=
+                  rec reduce fn (appstack args (App_l (mkApps (tConstruct ind n ui) l) :: ρ))
+                } ;
+              | view_other t ht with inspect (decompose_stack ρ') := {
+                | @exist (l, θ) eq4 :=
+                  give (tFix mfix idx) (appstack args (App_l (mkApps t l) :: ρ))
+                }
+              }
+            } ;
+          | _ := give (tFix mfix idx) π
+          } ;
+        | _ := give (tFix mfix idx) π
+        } ;
+      | false := give (tFix mfix idx) π
+      } ;
+
+    | red_view_Case ci p c brs π with RedFlags.iota flags := {
+      | true with inspect (reduce c (Case_discr ci p brs :: π) _) := {
+        | @exist (@exist (t,π') prf) eq with inspect (decompose_stack π') := {
+          | @exist (args, ρ) prf' with cc_viewc t := {
+            | ccview_construct ind' c' inst' with inspect (nth_error brs c') := {
+              | exist (Some br) eqbr := rec reduce (iota_red ci.(ci_npar) p args br) π ;
+              | exist None bot := False_rect _ _ } ;
+            | ccview_cofix mfix idx with inspect (unfold_cofix mfix idx) := {
+              | @exist (Some (narg, fn)) eq' :=
+                rec reduce (tCase ci p (mkApps fn args) brs) π ;
+              | @exist None bot := False_rect _ _
+              } ;
+            | ccview_other t ht := give (tCase ci p (mkApps t args) brs) π
+            }
+          }
+        } ;
+      | false := give (tCase ci p c brs) π
+      } ;
+
+    | red_view_Proj p c π with RedFlags.iota flags := {
+      | true with inspect (reduce c (Proj p :: π) _) := {
+        | @exist (@exist (t,π') prf) eq with inspect (decompose_stack π') := {
+          | @exist (args, ρ) prf' with cc0_viewc t := {
+            | cc0view_construct ind' _
+              with inspect (nth_error args (p.(proj_npars) + p.(proj_arg))) := {
+              | @exist (Some arg) eqa := rec reduce arg π ;
+              | @exist None eqa := False_rect _ _
+              } ;
+            | cc0view_cofix mfix idx with inspect (unfold_cofix mfix idx) := {
+              | @exist (Some (rarg, fn)) eq' :=
+                rec reduce (tProj p (mkApps fn args)) π ;
+              | @exist None bot := False_rect _ _
+              } ;
+            | cc0view_other t ht := give (tProj p (mkApps t args)) π
+            }
+          }
+        } ;
+      | false := give (tProj p c) π
+      } ;
+
+    | red_view_other t π discr := give t π
+
+    }.
+Admit Obligations.
+Admit Obligations.
+Admit Obligations.
+Admit Obligations.
+Admit Obligations.
+Admit Obligations.
+Admit Obligations.
+Admit Obligations.
+Admit Obligations.
+Admit Obligations.
+Admit Obligations.
+Admit Obligations.
+Admit Obligations.
+Admit Obligations.
+Admit Obligations.
+Admit Obligations.
+Admit Obligations.
+Admit Obligations.
+Admit Obligations.
+Admit Obligations.
+Admit Obligations.
+Admit Obligations.
+Admit Obligations.
+Admit Obligations.
+Admit Obligations.
+Admit Obligations.
+Admit Obligations.
+Admit Obligations.
+Admit Obligations.
+Admit Obligations.
+
+  Lemma welltyped_R_pres Σ (wfΣ : abstract_env_ext_rel X Σ) Γ :
+    forall x y : term × stack, welltyped Σ Γ (zip x) -> R Σ Γ y x -> welltyped Σ Γ (zip y).
+Admitted.
+
+  Section reducewf.
+    Context (Γ : context).
+
+    Notation sigmaarg :=
+      (sigma (fun t => sigma (fun π => forall Σ, abstract_env_ext_rel X Σ -> welltyped Σ Γ (zipc t π)))).
+
+    Local Instance wf_proof : WellFounded (fun x y : sigmaarg =>
+        forall Σ, abstract_env_ext_rel X Σ -> R Σ Γ (pr1 x, pr1 (pr2 x)) (pr1 y, pr1 (pr2 y))).
+    Proof using normalization_in.
+      intros [t [π wt]].
+       
+      unshelve eapply (Acc_intro_generator
+        (R:=fun x y : sigmaarg => forall Σ (wfΣ : abstract_env_ext_rel X Σ), R Σ Γ (x.(pr1), x.(pr2).(pr1)) (y.(pr1), y.(pr2).(pr1)))
+        (P:=fun x : sigmaarg => forall Σ (wfΣ : abstract_env_ext_rel X Σ), welltyped Σ Γ (zip (x.(pr1), x.(pr2).(pr1))))
+        (fun x y Px Hy => _) 1000 _ {| pr1 := t; pr2 := {| pr1 := π; pr2 := wt |} |} wt).
+      -
+ cbn in *.
+intros.
+destruct y as [t' [π' wt']].
+cbn.
+now apply wt'.
+      -
+ cbn in *.
+intros.
+        destruct (abstract_env_ext_exists X) as [[Σ wfΣ]].
+        destruct (hΣ _ wfΣ) as [hΣ].
+pose proof (R_Acc Γ (t0.(pr1), t0.(pr2).(pr1)) H).
+        clear -H0.
+destruct t0 as [t [π wt]].
+        cbn in *.
+revert wt.
+        depind H0.
+intros wt.
+constructor.
+intros.
+eapply H0.
+        *
+ cbn in H1.
+exact H1.
+        *
+ reflexivity.
+  Defined.
+
+  Equations reduce_stack_full (t : term) (π : stack) (h : forall Σ (wfΣ : abstract_env_ext_rel X Σ), welltyped Σ Γ (zip (t,π))) :
+    { t' : term * stack | forall Σ (wfΣ : abstract_env_ext_rel X Σ), Req Σ Γ t' (t, π) /\ Pr t' π /\ Pr' t' }
+    by wf (t, π) (fun (x y : term * stack) => forall Σ (wfΣ : abstract_env_ext_rel X Σ), R Σ Γ x y) :=
+    reduce_stack_full t π h := _reduce_stack Γ t π h (fun t' π' hr => reduce_stack_full t' π' (fun Σ wfΣ' => welltyped_R_pres Σ wfΣ' Γ _ _ (h Σ wfΣ') (hr Σ wfΣ'))).
+
+  End reducewf.
+
+  Definition reduce_stack Γ t π h :=
+    let '(exist ts _) := reduce_stack_full Γ t π h in ts.
+
+  Lemma reduce_stack_Req :
+    forall Σ (wfΣ : abstract_env_ext_rel X Σ) Γ t π h,
+     Req Σ Γ (reduce_stack Γ t π h) (t, π).
+Admitted.
+
+  Theorem reduce_stack_sound :
+    forall Σ (wfΣ : abstract_env_ext_rel X Σ) Γ t π h,
+      ∥ Σ ;;; Γ ⊢ zip (t, π) ⇝ zip (reduce_stack Γ t π h) ∥.
+Admitted.
+
+  Lemma reduce_stack_decompose :
+    forall Γ t π h,
+      snd (decompose_stack (snd (reduce_stack Γ t π h))) =
+      snd (decompose_stack π).
+Admitted.
+
+  Lemma reduce_stack_context :
+    forall Γ t π h,
+      stack_context (snd (reduce_stack Γ t π h)) =
+      stack_context π.
+Admitted.
+
+  Definition isred (t : term * stack) :=
+    isApp (fst t) = false /\
+    (isLambda (fst t) -> isStackApp (snd t) = false).
+
+  Lemma reduce_stack_isred :
+    forall Γ t π h,
+      RedFlags.beta flags ->
+      isred (reduce_stack Γ t π h).
+Admitted.
+
+  Lemma reduce_stack_noApp :
+    forall Γ t π h,
+      isApp (fst (reduce_stack Γ t π h)) = false.
+Admitted.
+
+  Lemma reduce_stack_noLamApp :
+    forall Γ t π h,
+      RedFlags.beta flags ->
+      isLambda (fst (reduce_stack Γ t π h)) ->
+      isStackApp (snd (reduce_stack Γ t π h)) = false.
+Admitted.
+
+  Definition reduce_term Γ t
+    (h : forall Σ, abstract_env_ext_rel X Σ -> welltyped Σ Γ t) :=
+    zip (reduce_stack Γ t [] h).
+
+  Theorem reduce_term_sound :
+    forall Γ t (h : forall Σ, abstract_env_ext_rel X Σ -> welltyped Σ Γ t)
+      Σ, abstract_env_ext_rel X Σ ->
+      ∥ Σ ;;; Γ ⊢ t ⇝ reduce_term Γ t h ∥.
+Admitted.
+
+  Scheme Acc_ind' := Induction for Acc Sort Prop.
+
+  Lemma Fix_F_prop :
+    forall A R P f (pred : forall x : A, P x -> Prop) x hx,
+      (forall x aux, (forall y hy, pred y (aux y hy)) -> pred x (f x aux)) ->
+      pred x (@Fix_F A R P f x hx).
+Admitted.
+
+  Lemma reduce_stack_prop :
+    forall Γ t π h (P : term × stack -> term × stack -> Prop),
+      (forall t π h aux,
+          (forall t' π' hR, P (t', π') (` (aux t' π' hR))) ->
+          P (t, π) (` (_reduce_stack Γ t π h aux))) ->
+      P (t, π) (reduce_stack Γ t π h).
+Admitted.
+
+  Lemma decompose_stack_at_appstack_None l s n :
+    isStackApp s = false ->
+    nth_error l n = None <->
+    decompose_stack_at (appstack l s) n = None.
+Admitted.
+
+  Lemma mkApps_tApp hd arg args :
+    mkApps (tApp hd arg) args = mkApps hd (arg :: args).
+Admitted.
+
+  Lemma tApp_mkApps hd args arg :
+    tApp (mkApps hd args) arg = mkApps hd (args ++ [arg]).
+Admitted.
+
+  Lemma whnf_non_ctor_finite_ind_typed Σ Γ t ind u args :
+    wf Σ ->
+    whnf flags Σ Γ t ->
+    isConstruct_app t = false ->
+    check_recursivity_kind (lookup_env Σ) (inductive_mind ind) CoFinite = false ->
+    Σ ;;; Γ |- t : mkApps (tInd ind u) args ->
+    whne flags Σ Γ t.
+Admitted.
+
+  Definition isCoFix_app t :=
+    match (decompose_app t).1 with
+    | tCoFix _ _ => true
+    | _ => false
+    end.
+
+  Lemma whnf_non_ctor_non_cofix_ind_typed Σ Γ t ind u args :
+    wf Σ ->
+    whnf flags Σ Γ t ->
+    isConstruct_app t = false ->
+    isCoFix_app t = false ->
+    Σ ;;; Γ |- t : mkApps (tInd ind u) args ->
+    whne flags Σ Γ t.
+Admitted.
+
+  Lemma whnf_fix_arg_whne mfix idx body Σ Γ t before args aftr ty :
+    wf Σ ->
+    unfold_fix mfix idx = Some (#|before|, body) ->
+    match t with
+    | tConstruct _ _ _ => False
+    | tApp _ _ => False
+    | _ => True
+    end ->
+    whnf flags Σ Γ (mkApps t args) ->
+    Σ ;;; Γ |- mkApps (tFix mfix idx) (before ++ mkApps t args :: aftr) : ty ->
+    whne flags Σ Γ (mkApps t args).
+Admitted.
+
+  Lemma whnf_case_arg_whne Σ Γ hd args ci p brs T :
+    wf Σ ->
+    match hd with
+    | tApp _ _
+    | tConstruct _ _ _
+    | tCoFix _ _ => False
+    | _ => True
+    end ->
+    whnf flags Σ Γ (mkApps hd args) ->
+    Σ;;; Γ |- tCase ci p (mkApps hd args) brs : T ->
+    whne flags Σ Γ (mkApps hd args).
+Admitted.
+
+  Lemma whnf_proj_arg_whne Σ Γ hd args p T :
+    wf Σ ->
+    match hd with
+    | tApp _ _
+    | tCoFix _ _ => False
+    | tConstruct _ c _ => c <> 0
+    | _ => True
+    end ->
+    whnf flags Σ Γ (mkApps hd args) ->
+    Σ ;;; Γ |- tProj p (mkApps hd args) : T ->
+    whne flags Σ Γ (mkApps hd args).
+Admitted.
+
+  Lemma reduce_stack_whnf :
+    forall Γ t π h Σ (wfΣ : abstract_env_ext_rel X Σ),
+      let '(u, ρ) := reduce_stack Γ t π h in
+       ∥whnf flags Σ (Γ ,,, stack_context ρ) (zipp u ρ)∥.
+Admitted.
+
+  Theorem reduce_term_complete Σ (wfΣ : abstract_env_ext_rel X Σ) Γ t h :
+    ∥whnf flags Σ Γ (reduce_term Γ t h)∥.
+Admitted.
+
+End Reduce.
+
+Section ReduceFns.
+
+  Context {cf : checker_flags} {no : normalizing_flags}
+          {X_type : abstract_env_impl} {X : X_type.π2.π1} {normalization_in : forall Σ, wf_ext Σ -> Σ ∼_ext X -> NormalizationIn Σ}.
+
+   
+  Opaque reduce_stack_full.
+
+  Definition hnf := reduce_term RedFlags.default X_type X.
+
+  Theorem hnf_sound {Γ t h} Σ (wfΣ : abstract_env_ext_rel X Σ) : ∥ Σ ;;; Γ ⊢ t ⇝ hnf Γ t h ∥.
+  Proof using Type.
+    unfold hnf.
+    destruct (reduce_term_sound RedFlags.default _ X _ _ h Σ wfΣ).
+    sq.
+eapply into_closed_red; fvs.
+  Defined.
+
+  Theorem hnf_complete {Γ t h} Σ (wfΣ : abstract_env_ext_rel X Σ) : ∥whnf RedFlags.default Σ Γ (hnf Γ t h)∥.
+Admitted.
+
+  Equations? reduce_to_sort (Γ : context) (t : term)
+    (h : forall Σ (wfΣ : abstract_env_ext_rel X Σ), welltyped Σ Γ t)
+    : typing_result_comp (∑ u, forall Σ (wfΣ : abstract_env_ext_rel X Σ), ∥ Σ ;;; Γ ⊢ t ⇝ tSort u ∥) :=
+    reduce_to_sort Γ t h with view_sortc t := {
+      | view_sort_sort s => Checked_comp (s; _);
+      | view_sort_other t _ with inspect (hnf Γ t h) :=
+        | exist hnft eq with view_sortc hnft := {
+          | view_sort_sort s => Checked_comp (s; _);
+          | view_sort_other hnft r => TypeError_comp (NotASort hnft) _
+        }
+      }.
+  Proof using Type.
+    *
+ destruct (h _ wfΣ) as [? hs].
+      pose proof (hΣ := hΣ _ X _ wfΣ).
+sq.
+      eapply (wt_closed_red_refl hs).
+    *
+ pose proof (hnf_sound (h:=h)).
+      now rewrite eq.
+    *
+ destruct (abstract_env_ext_exists X) as [[Σ wfΣ]].
+specialize (X1 _ wfΣ).
+      pose proof (hΣ := hΣ _ X _ wfΣ).
+sq.
+      pose proof (@hnf_complete Γ t h) as [wh]; eauto.
+      pose proof (@hnf_sound Γ t h) as [r']; eauto.
+      eapply PCUICContextConversion.closed_red_confluence in X1 as (?&r1&r2); eauto.
+      apply invert_red_sort in r2 as ->.
+      eapply whnf_red_inv in r1; eauto.
+      depelim r1.
+      rewrite H in r.
+      now cbn in r.
+  Qed.
+
+  Lemma reduce_to_sort_complete {Γ t wt} Σ (wfΣ : abstract_env_ext_rel X Σ)
+    e p :
+    reduce_to_sort Γ t wt = TypeError_comp e p ->
+    (forall s, red Σ Γ t (tSort s) -> False).
+Admitted.
+
+  Equations? reduce_to_prod (Γ : context) (t : term)
+    (h : forall Σ (wfΣ : abstract_env_ext_rel X Σ), welltyped Σ Γ t)
+    : typing_result_comp (∑ na a b, forall  Σ (wfΣ : abstract_env_ext_rel X Σ), ∥ Σ ;;; Γ ⊢ t ⇝ tProd na a b ∥) :=
+    reduce_to_prod Γ t h with view_prodc t := {
+      | view_prod_prod na a b => Checked_comp (na; a; b; _);
+      | view_prod_other t _ with inspect (hnf Γ t h) :=
+        | exist hnft eq with view_prodc hnft := {
+          | view_prod_prod na a b => Checked_comp (na; a; b; _);
+          | view_prod_other hnft _ => TypeError_comp (NotAProduct t hnft) _
+        }
+      }.
+  Proof using Type.
+    *
+ destruct (h _ wfΣ) as [? hs].
+      pose proof (hΣ := hΣ _ _ _ wfΣ).
+sq.
+      now eapply wt_closed_red_refl.
+    *
+ pose proof (hnf_sound (h:=h)).
+      now rewrite eq.
+    *
+ destruct (abstract_env_ext_exists X) as [[Σ wfΣ]].
+      specialize (X3 _ wfΣ).
+      sq.
+      pose proof (@hnf_complete Γ t h) as [wh]; eauto.
+      pose proof (@hnf_sound Γ t h) as [r']; eauto.
+      destruct (hΣ _ _ _ wfΣ).
+      eapply PCUICContextConversion.closed_red_confluence in X3 as (?&r1&r2); eauto.
+      apply invert_red_prod in r2 as (?&?&[-> ? ?]); auto.
+      eapply whnf_red_inv in r1; auto.
+      depelim r1.
+      now rewrite H in n0.
+  Qed.
+
+  Lemma reduce_to_prod_complete {Γ t wt} Σ (wfΣ : abstract_env_ext_rel X Σ)
+    e p :
+    reduce_to_prod Γ t wt = TypeError_comp e p ->
+    (forall na a b, red Σ Γ t (tProd na a b) -> False).
+Admitted.
+
+  Equations? reduce_to_ind (Γ : context) (t : term)
+    (h : forall Σ (wfΣ : abstract_env_ext_rel X Σ), welltyped Σ Γ t)
+    : typing_result_comp (∑ i u l, forall Σ (wfΣ : abstract_env_ext_rel X Σ), ∥ Σ ;;; Γ ⊢ t ⇝ mkApps (tInd i u) l ∥) :=
+    reduce_to_ind Γ t h with inspect (decompose_app t) := {
+      | exist (thd, args) eq_decomp with view_indc thd := {
+        | view_ind_tInd i u => Checked_comp (i; u; args; _);
+        | view_ind_other thd _ with inspect (reduce_stack RedFlags.default _ X Γ t [] h) := {
+          | exist (hnft, π) eq with view_indc hnft := {
+            | view_ind_tInd i' u with inspect (decompose_stack π) := {
+              | exist (l, _) eq_decomp' => Checked_comp (i'; u; l; _)
+              };
+            | view_ind_other _ _ => TypeError_comp (NotAnInductive t) _
+            }
+          }
+        }
+      }.
+  Proof using Type.
+    -
+ specialize (h _ wfΣ).
+destruct h  as [? h].
+      assert (Xeq : mkApps (tInd i u) args = t).
+      {
+ etransitivity.
+2: symmetry; eapply mkApps_decompose_app.
+        now rewrite <- eq_decomp.
+}
+      rewrite Xeq.
+pose proof (hΣ := hΣ _ _ _ wfΣ); sq; eapply (wt_closed_red_refl h).
+    -
+ pose proof (reduce_stack_sound RedFlags.default _ X _ wfΣ _ _ [] h).
+      rewrite <- eq in H.
+      cbn in *.
+      assert (π = appstack l []) as ->.
+      2: {
+ now rewrite zipc_appstack in H.
+}
+      unfold reduce_stack in eq.
+      destruct reduce_stack_full as (?&_&stack_val&?); eauto.
+      subst x.
+      unfold Pr in stack_val.
+      cbn in *.
+      assert (decomp: decompose_stack π = ((decompose_stack π).1, [])).
+      {
+ rewrite stack_val.
+        now destruct decompose_stack.
+}
+      apply decompose_stack_eq in decomp as ->.
+      now rewrite <- eq_decomp'.
+    -
+ destruct (abstract_env_ext_exists X) as [[Σ wfΣ]].
+      specialize (X3 _ wfΣ).
+      pose proof (hΣ := hΣ _ _ _ wfΣ).
+sq.
+      pose proof (reduce_stack_whnf RedFlags.default _ X Γ t [] h _  wfΣ) as wh.
+      unfold reduce_stack in *.
+      destruct reduce_stack_full as ((hd&π')&r'&stack_valid&(notapp&_)); eauto.
+      destruct wh as [wh].
+      apply Req_red in r' as [r'].
+      unfold Pr in stack_valid.
+      cbn in *.
+      eapply into_closed_red in r'; fvs.
+      eapply PCUICContextConversion.closed_red_confluence in r' as (?&r1&r2).
+      2 : exact X3.
+      assert (exists args, π' = appstack args []) as (?&->).
+      {
+ exists ((decompose_stack π').1).
+        assert (decomp: decompose_stack π' = ((decompose_stack π').1, [])).
+        {
+ now rewrite stack_valid; destruct decompose_stack; cbn.
+}
+        now apply decompose_stack_eq in decomp.
+}
+      unfold zipp in wh.
+      rewrite stack_context_appstack, decompose_stack_appstack in wh.
+      rewrite zipc_appstack in r2.
+      cbn in *.
+      rewrite app_nil_r in wh.
+      eapply whnf_red_inv in r2; eauto.
+      apply invert_red_mkApps_tInd in r1 as (?&[-> _ ?]); auto.
+      apply whnf_red_mkApps_inv in r2 as (?&?); auto.
+      depelim w.
+      noconf eq.
+      discriminate i0.
+  Qed.
+
+  Lemma reduce_to_ind_complete  Σ (wfΣ : abstract_env_ext_rel X Σ) Γ ty wat e p :
+    reduce_to_ind Γ ty wat = TypeError_comp e p ->
+    forall ind u args,
+      red Σ Γ ty (mkApps (tInd ind u) args) ->
+      False.
+Admitted.
+
+   
+  Definition arity_ass := aname * term.
+
+  Fixpoint mkAssumArity (l : list arity_ass) (s : Universe.t) : term :=
+    match l with
+    | [] => tSort s
+    | (na, A) :: l => tProd na A (mkAssumArity l s)
+    end.
+
+  Definition arity_ass_context := rev_map (fun '(na, A) => vass na A).
+
+  Lemma assumption_context_arity_ass_context l :
+    assumption_context (arity_ass_context l).
+Admitted.
+
+  Lemma mkAssumArity_it_mkProd_or_LetIn (l : list arity_ass) (s : Universe.t) :
+    mkAssumArity l s = it_mkProd_or_LetIn (arity_ass_context l) (tSort s).
+Admitted.
+
+  Lemma isArity_mkAssumArity l s :
+    isArity (mkAssumArity l s).
+Admitted.
+
+  Record conv_arity {Γ T} : Type :=
+    build_conv_arity {
+        conv_ar_context : list arity_ass;
+        conv_ar_univ : Universe.t;
+        conv_ar_red : forall Σ (wfΣ : abstract_env_ext_rel X Σ), ∥ Σ ;;; Γ ⊢ T ⇝ mkAssumArity conv_ar_context conv_ar_univ ∥
+      }.
+
+  Global Arguments conv_arity : clear implicits.
+
+  Lemma conv_arity_Is_conv_to_Arity {Γ T} :
+    is_closed_context Γ ->
+    is_open_term Γ T ->
+    conv_arity Γ T ->
+    forall Σ (wfΣ : abstract_env_ext_rel X Σ), Is_conv_to_Arity Σ Γ T.
+Admitted.
+
+  Lemma isArity_red Σ Γ u v :
+    isArity u ->
+    red Σ Γ u v ->
+    isArity v.
+Admitted.
+
+  Lemma Is_conv_to_Arity_red Σ {wfΣ : wf Σ} Γ T T' :
+    Is_conv_to_Arity Σ Γ T ->
+    Σ ;;; Γ ⊢ T ⇝ T' ->
+    Is_conv_to_Arity Σ Γ T'.
+Admitted.
+
+  Local Instance wellfounded Σ wfΣ {normalization:NormalizationIn Σ} : WellFounded (@hnf_subterm_rel _ Σ) :=
+    @wf_hnf_subterm _ _ _ normalization (heΣ _ X Σ wfΣ).
+
+End ReduceFns.
+
+End PCUICSafeReduce.
+
+End MetaCoq_DOT_SafeChecker_DOT_PCUICSafeReduce_WRAPPED.
+Module Export MetaCoq_DOT_SafeChecker_DOT_PCUICSafeReduce.
+Module Export MetaCoq.
+Module Export SafeChecker.
+Module PCUICSafeReduce.
+Include MetaCoq_DOT_SafeChecker_DOT_PCUICSafeReduce_WRAPPED.PCUICSafeReduce.
+End PCUICSafeReduce.
+
+End SafeChecker.
+
+End MetaCoq.
+
+End MetaCoq_DOT_SafeChecker_DOT_PCUICSafeReduce.
+Require MetaCoq.PCUIC.PCUICConvCumInversion.
+Axiom proof_admitted : False.
+Tactic Notation "admit" := abstract case proof_admitted.
+Import MetaCoq.Utils.utils.
+Import MetaCoq.Common.config.
+Import MetaCoq.PCUIC.PCUICAst.
+Import MetaCoq.PCUIC.PCUICTyping.
+Import MetaCoq.PCUIC.PCUICConversion.
+Import MetaCoq.PCUIC.PCUICNormal.
+Import MetaCoq.PCUIC.Syntax.PCUICPosition.
+Import MetaCoq.PCUIC.PCUICSN.
+Import MetaCoq.PCUIC.PCUICWellScopedCumulativity.
+Import MetaCoq.PCUIC.PCUICConvCumInversion.
+Import MetaCoq.SafeChecker.PCUICErrors.
+Import MetaCoq.SafeChecker.PCUICWfEnv.
+Import MetaCoq.SafeChecker.PCUICSafeReduce.
+
+  Context {cf : checker_flags} {nor : normalizing_flags}.
+
+  Context (X_type : abstract_env_impl).
+
+  Context (X : X_type.π2.π1).
 
   Inductive state :=
   | Reduction
@@ -290,22 +1059,8 @@ Section Conversion.
   | Args
   | Fallback.
 
-  Inductive stateR : state -> state -> Prop :=
-  | stateR_Term_Reduction : stateR Term Reduction
-  | stateR_Args_Term : stateR Args Term
-  | stateR_Fallback_Term : stateR Fallback Term
-  | stateR_Args_Fallback : stateR Args Fallback.
-
-  Derive Signature for stateR.
-
-  Lemma stateR_Acc :
-    forall s, Acc stateR s.
-Admitted.
-
   Notation wtp Γ t π :=
     (forall Σ (wfΣ : abstract_env_ext_rel X Σ), welltyped Σ Γ (zipc t π)) (only parsing).
-
-  Set Primitive Projections.
 
   Record pack (Γ : context) := mkpack {
     st   : state ;
@@ -325,44 +1080,9 @@ Admitted.
 
   Definition wterm Γ := { t : term | forall Σ (wfΣ : abstract_env_ext_rel X Σ), welltyped Σ Γ t }.
 
-  Definition wcored Γ (u v : wterm Γ) :=
-    forall Σ (wfΣ : abstract_env_ext_rel X Σ), cored' Σ Γ (` u) (` v).
-
-  Lemma wcored_wf :
-    forall Γ, well_founded (wcored Γ).
-Admitted.
-
-  Import MetaCoq.PCUIC.PCUICAlpha.
-
-  Definition eqt u v := ∥ u ≡α v ∥.
-
-  Lemma eqt_eqterm {Σ} {wfΣ : abstract_env_ext_rel X Σ} {u v} :
-    u ≡α v -> eq_term Σ Σ u v.
-Admitted.
-
-  Local Instance eqt_refl : RelationClasses.Reflexive eqt.
-Admitted.
-
-  Lemma eq_term_valid_pos :
-    forall {u v p},
-      validpos u p ->
-      eqt u v ->
-      validpos v p.
-Admitted.
-
-  Definition weqt {Γ} (u v : wterm Γ) :=
-    eqt (` u) (` v).
-
   Lemma R_aux (Γ : context) :
     (∑ t : term, pos t × (∑ w : wterm Γ, pos (` w) × state)) ->
-    (∑ t : term, pos t × (∑ w : wterm Γ, pos (` w) × state)) -> Prop. Admitted.
-
-  Derive Signature for Subterm.lexprod.
-
-  Lemma R_aux_Acc :
-    forall Γ t p w q s,
-      (forall Σ, abstract_env_ext_rel X Σ -> welltyped Σ Γ t) ->
-      Acc (R_aux Γ) (t ; (p, (w ; (q, s)))).
+    (∑ t : term, pos t × (∑ w : wterm Γ, pos (` w) × state)) -> Prop.
 Admitted.
 
   Notation pzt u := (zipc (tm1 u) (stk1 u)) (only parsing).
@@ -377,132 +1097,11 @@ Admitted.
   Definition R Γ (u v : pack Γ) :=
     R_aux Γ (obpack u) (obpack v).
 
-  Lemma R_Acc :
-    forall Γ u,
-      (forall Σ (wfΣ : abstract_env_ext_rel X Σ), welltyped Σ Γ (zipc (tm1 u) (stk1 u))) ->
-      Acc (R Γ) u.
-Admitted.
-
-  Notation eq_term Σ t u := (eq_term Σ Σ t u).
-
-  Lemma R_aux_irrelevance Γ x y z :
-    ((x.π1; x.π2.1), (existT (fun x => pos x × state) (` x.π2.2.π1) x.π2.2.π2)) =
-    ((y.π1; y.π2.1), (existT (fun x => pos x × state) (` y.π2.2.π1) y.π2.2.π2)) ->
-    R_aux Γ z x -> R_aux Γ z y.
-Admitted.
-
-  Lemma R_irrelevance Γ x y z :
-    (x.(st), x.(tm1), x.(stk1), x.(tm2), x.(stk2)) =
-    (y.(st), y.(tm1), y.(stk1), y.(tm2), y.(stk2)) ->
-    R Γ z x -> R Γ z y.
-Admitted.
-
-  Lemma R_cored :
-    forall Γ p1 p2,
-      (forall Σ (wfΣ : abstract_env_ext_rel X Σ), cored Σ Γ (pzt p1) (pzt p2)) ->
-      R Γ p1 p2.
-Admitted.
-
-  Lemma R_aux_positionR :
-    forall Γ t1 t2 (p1 : pos t1) (p2 : pos t2) s1 s2,
-      eqt t1 t2 ->
-      positionR (` p1) (` p2) ->
-      R_aux Γ (t1 ; (p1, s1)) (t2 ; (p2, s2)).
-Admitted.
-
-  Lemma R_positionR :
-    forall Γ p1 p2,
-      (eqt (pzt p1) (pzt p2)) ->
-      positionR (` (pps1 p1)) (` (pps1 p2)) ->
-      R Γ p1 p2.
-Admitted.
-
-  Lemma R_aux_cored2 :
-    forall Γ t1 t2 (p1 : pos t1) (p2 : pos t2) w1 w2 q1 q2 s1 s2,
-      (eqt t1 t2) ->
-      ` p1 = ` p2 ->
-      (forall Σ (wfΣ : abstract_env_ext_rel X Σ), cored' Σ Γ (` w1) (` w2)) ->
-      R_aux Γ (t1 ; (p1, (w1 ; (q1, s1)))) (t2 ; (p2, (w2 ; (q2, s2)))).
-Admitted.
-
-  Lemma R_cored2 :
-    forall Γ p1 p2,
-      (eqt (pzt p1) (pzt p2)) ->
-      ` (pps1 p1) = ` (pps1 p2) ->
-      (forall Σ (wfΣ : abstract_env_ext_rel X Σ),
-          cored Σ Γ (` (pwt p1)) (` (pwt p2))) ->
-      R Γ p1 p2.
-Admitted.
-
-  Lemma R_aux_positionR2 :
-    forall Γ t1 t2 (p1 : pos t1) (p2 : pos t2) w1 w2 q1 q2 s1 s2,
-      (eqt t1 t2) ->
-      ` p1 = ` p2 ->
-      (eqt (` w1) (` w2)) ->
-      positionR (` q1) (` q2) ->
-      R_aux Γ (t1 ; (p1, (w1 ; (q1, s1)))) (t2 ; (p2, (w2 ; (q2, s2)))).
-Admitted.
-
-  Lemma R_positionR2 :
-    forall Γ p1 p2,
-      (eqt (pzt p1) (pzt p2)) ->
-      ` (pps1 p1) = ` (pps1 p2) ->
-      (eqt (` (pwt p1)) (` (pwt p2))) ->
-      positionR (` (pps2 p1)) (` (pps2 p2)) ->
-      R Γ p1 p2.
-Admitted.
-
-  Lemma R_aux_stateR :
-    forall Γ t1 t2 (p1 : pos t1) (p2 : pos t2) w1 w2 q1 q2 s1 s2 ,
-      (eqt t1 t2) ->
-      ` p1 = ` p2 ->
-      (eqt (` w1) (` w2)) ->
-      ` q1 = ` q2 ->
-      stateR s1 s2 ->
-      R_aux Γ (t1 ; (p1, (w1 ; (q1, s1)))) (t2 ; (p2, (w2 ; (q2, s2)))).
-Admitted.
-
-  Lemma R_stateR :
-    forall Γ p1 p2,
-      (eqt (pzt p1) (pzt p2)) ->
-      ` (pps1 p1) = ` (pps1 p2) ->
-      (eqt (` (pwt p1)) (` (pwt p2))) ->
-      ` (pps2 p1) = ` (pps2 p2) ->
-      stateR (st p1) (st p2) ->
-      R Γ p1 p2.
-Admitted.
-
-  Definition abstract_env_compare_global_instance := compare_global_instance (abstract_env_lookup X) (abstract_env_eq X).
-
-  Notation eqb_ctx := (eqb_ctx_gen (abstract_env_eq X) abstract_env_compare_global_instance).
-  Notation eqb_term := (eqb_term_upto_univ (abstract_env_eq X) (abstract_env_eq X) abstract_env_compare_global_instance).
-  Notation leqb_term := (eqb_term_upto_univ (abstract_env_eq X) (abstract_env_leq X) abstract_env_compare_global_instance).
-
-  Definition eqb_term_stack t1 π1 t2 π2 :=
-    eqb_ctx (stack_context π1) (stack_context π2) &&
-    eqb_term (zipp t1 π1) (zipp t2 π2).
-
-  Lemma iff_reflect (P : Prop) (b : bool) :
-    P <-> b -> reflect P b.
-Admitted.
-
-  Definition wf_universe_iff  Σ u :
-    wf_universeb Σ u <-> wf_universe Σ u.
-Admitted.
-
-  Definition wf_universe_instance_iff  Σ u :
-    wf_universeb_instance Σ u <-> wf_universe_instance Σ u.
-Admitted.
-
   Notation conv_stack_ctx Γ π1 π2 :=
     (forall Σ, abstract_env_ext_rel X Σ -> ∥ (Σ ⊢ Γ ,,, stack_context π1 = Γ ,,, stack_context π2) ∥).
 
   Notation conv_term leq Γ t π t' π' :=
     (forall Σ, abstract_env_ext_rel X Σ -> conv_cum leq Σ (Γ ,,, stack_context π) (zipp t π) (zipp t' π'))
-      (only parsing).
-
-  Notation alt_conv_term Γ t π t' π' :=
-    (forall Σ, abstract_env_ext_rel X Σ -> ∥ Σ ;;; Γ ,,, stack_context π ⊢ zipp t π = zipp t' π' ∥)
       (only parsing).
 
   Inductive ConversionResult (P : Prop) :=
@@ -516,126 +1115,8 @@ Admitted.
     isApp t = false /\
     forall Σ, abstract_env_ext_rel X Σ -> ∥whnf RedFlags.nodelta Σ (Γ,,, stack_context π) (zipp t π)∥.
 
-  Lemma isred_full_nobeta Γ t π :
-    isred_full Γ t π ->
-    isLambda t ->
-    isStackApp π = false.
+  Lemma prog_discr (t1 t2 : term) : Prop.
 Admitted.
-
-  Lemma eta_pair {A B} (p q : A * B) :
-    p = q ->
-    (p.1, p.2) = (q.1, q.2).
-Admitted.
-
-  Ltac is_var t :=
-    match goal with
-    | v : _ |- _ =>
-      match t with
-      | v => idtac
-      end
-    end.
-
-  Lemma zipp_stack_cat_decompose_stack t π π' :
-    zipp t (π ++ (decompose_stack π').2) = zipp t π.
-Admitted.
-
-  Lemma zipc_decompose_stack_empty t π :
-    (decompose_stack π).2 = [] ->
-    zipc t π = zipp t π.
-Admitted.
-
-  Ltac reduce_stack_facts Σ wfΣ :=
-    repeat
-      match goal with
-      | [H: (?a, ?b) = reduce_stack ?f _ ?X ?Γ ?t ?π ?h |- _] =>
-        let rid := fresh "r" in
-        let decompid := fresh "d" in
-        let whid := fresh "w" in
-        let isr := fresh "isr" in
-        pose proof (reduce_stack_sound f _ X Σ wfΣ Γ t π h) as [rid];
-        pose proof (reduce_stack_decompose f _ X Γ t π h) as decompid;
-        pose proof (reduce_stack_whnf f _ X Γ t π h Σ wfΣ) as whid;
-        pose proof (reduce_stack_isred f _ X Γ t π h) as isr;
-        rewrite <- H in rid, decompid, whid, isr; cbn in rid, decompid, whid, isr;
-        clear H
-      end.
-
-  Lemma zipc_unfold_decompose_stack t π :
-    zipc t π = zipc (mkApps t (decompose_stack π).1) (decompose_stack π).2.
-Admitted.
-
-  Ltac simpl_stacks :=
-    (repeat
-       match goal with
-       | [H: (?a, ?b) = decompose_stack ?π |- _] =>
-         is_var a;
-         is_var b;
-         apply eta_pair in H; cbn in H; noconf H
-       end);
-    (repeat
-       match goal with
-       | [H: context[decompose_stack (appstack ?l ?ρ)] |- _] =>
-         (rewrite (decompose_stack_appstack l ρ) in H; cbn in H) || fail 2
-       | [H: context[stack_context (?π ++ ?π')] |- _] =>
-         (rewrite (stack_context_stack_cat π' π) in H; cbn in H) || fail 2
-       | [H: (decompose_stack ?π).2 = [], H': context[stack_context ?π] |- _] =>
-         (rewrite <- (stack_context_decompose π), H in H'; cbn in H') || fail 2
-       | [H: (decompose_stack ?π).2 = [], H': context[zipc ?t ?π] |- _] =>
-         (rewrite (zipc_decompose_stack_empty t π H) in H'; cbn in H') || fail 2
-       | [H: context[stack_context (decompose_stack ?π).2] |- _] =>
-         (rewrite (stack_context_decompose π) in H; cbn in H) || fail 2
-       | [H: context[zipp ?t (?π ++ (decompose_stack ?π').2)] |- _] =>
-         (rewrite (zipp_stack_cat_decompose_stack t π π') in H; cbn in H) || fail 2
-       | [H: context[zipc ?t (appstack ?args ?π)] |- _] =>
-         (rewrite (@zipc_appstack t args π) in H; cbn in H) || fail 2
-       | [H: context[zipc ?t (?π ++ ?π')] |- _] =>
-         (rewrite (zipc_stack_cat t π π') in H; cbn in H) || fail 2
-       | [H: context[zip (mkApps ?t (decompose_stack ?π).1, decompose_stack ?π).2] |- _] =>
-         unfold zip in H
-       | [H: context[zipc (mkApps ?t (decompose_stack ?π).1) (decompose_stack ?π).2] |- _] =>
-         (rewrite <- (zipc_unfold_decompose_stack t π) in H; cbn in H) || fail 2
-       | [H: isStackApp ?π = false, H': context[zipp ?t ?π] |- _] =>
-         (rewrite (zipp_noStackApp t π H) in H'; cbn in H') || fail 2
-       | [H: (decompose_stack ?π).2 = (decompose_stack ?π').2, H': context[stack_context ?π] |- _] =>
-         (rewrite <- (stack_context_decompose π), H, (stack_context_decompose π') in H'; cbn in H')
-         || fail 2
-
-       | [|- context[decompose_stack (appstack ?l ?ρ)]] =>
-         (rewrite (decompose_stack_appstack l ρ); cbn) || fail 2
-       | [|- context[stack_context (?π ++ ?π')]] =>
-         (rewrite (stack_context_stack_cat π' π); cbn) || fail 2
-       | [H: (decompose_stack ?π).2 = [] |- context[stack_context ?π]] =>
-         (rewrite <- (stack_context_decompose π), H; cbn) || fail 2
-       | [H: (decompose_stack ?π).2 = [] |- context[zipc ?t ?π]] =>
-         (rewrite (zipc_decompose_stack_empty t π H); cbn) || fail 2
-       | [|- context[stack_context (decompose_stack ?π).2]] =>
-         (rewrite (stack_context_decompose π); cbn) || fail 2
-       | [|- context[zipp ?t (?π ++ (decompose_stack ?π').2)]] =>
-         (rewrite (zipp_stack_cat_decompose_stack t π π'); cbn) || fail 2
-       | [|- context[zipc ?t (appstack ?args ?π)]] =>
-         (rewrite (@zipc_appstack t args π); cbn) || fail 2
-       | [|- context[zipc ?t (?π ++ ?π')]] =>
-         (rewrite (zipc_stack_cat t π π'); cbn) || fail 2
-       | [|- context[zip (mkApps ?t (decompose_stack ?π).1, decompose_stack ?π).2]] =>
-         unfold zip
-       | [|- context[zipc (mkApps ?t (decompose_stack ?π).1) (decompose_stack ?π).2]] =>
-         (rewrite <- (zipc_unfold_decompose_stack t π); cbn) || fail 2
-       | [H: isStackApp ?π = false |- context[zipp ?t ?π]] =>
-         (rewrite (zipp_noStackApp t π H); cbn) || fail 2
-       | [H: (decompose_stack ?π).2 = (decompose_stack ?π').2 |- context[stack_context ?π]] =>
-         (rewrite <- (stack_context_decompose π), H, (stack_context_decompose π'); cbn) || fail 2
-       end);
-    repeat
-      match goal with
-      | [H: context[zipp ?t ?π] |- _] => rewrite (zipp_as_mkApps t π) in H
-      | [|- context[zipp ?t ?π]] => rewrite (zipp_as_mkApps t π)
-      end.
-
-  Ltac simpl_reduce_stack Σ wfΣ := reduce_stack_facts Σ wfΣ ; simpl_stacks.
-
-
-  Lemma prog_discr (t1 t2 : term) : Prop. Admitted.
-
 
   Definition Ret s Γ t π t' π' :=
     forall (leq : conv_pb),
@@ -667,295 +1148,8 @@ Admitted.
   Local Notation yes := (Success _) (only parsing).
   Local Notation no := (fun e => Error e _) (only parsing).
 
-
-  Local Notation repack e :=
-    (match e with Success h => Success _ | Error er h => Error er _ end)
-    (only parsing).
-
   Notation isconv_red_raw leq t1 π1 t2 π2 aux :=
     (aux Reduction t1 π1 t2 π2 _ _ _ _ leq _ I I I) (only parsing).
-  Notation isconv_prog_raw leq t1 π1 t2 π2 aux :=
-    (aux Term t1 π1 t2 π2 _ _ _ _ leq _ _ _ I) (only parsing).
-  Notation isconv_args_raw leq t1 π1 t2 π2 aux :=
-    (aux Args t1 π1 t2 π2 _ _ _ _ leq _ I I I) (only parsing).
-  Notation isconv_fallback_raw leq t1 π1 t2 π2 aux :=
-    (aux Fallback t1 π1 t2 π2 _ _ _ _ leq _ _ _ _) (only parsing).
-
-  Notation isconv_red leq t1 π1 t2 π2 aux :=
-    (repack (isconv_red_raw leq t1 π1 t2 π2 aux)) (only parsing).
-  Notation isconv_prog leq t1 π1 t2 π2 aux :=
-    (repack (isconv_prog_raw leq t1 π1 t2 π2 aux)) (only parsing).
-  Notation isconv_args leq t1 π1 t2 π2 aux :=
-    (repack (isconv_args_raw leq t1 π1 t2 π2 aux)) (only parsing).
-  Notation isconv_fallback leq t1 π1 t2 π2 aux :=
-    (repack (isconv_fallback_raw leq t1 π1 t2 π2 aux)) (only parsing).
-
-  Lemma _isconv_red (Γ : context) (leq : conv_pb)
-            (t1 : term) (π1 : stack) (h1 : wtp Γ t1 π1)
-            (t2 : term) (π2 : stack) (h2 : wtp Γ t2 π2)
-            (hx : conv_stack_ctx Γ π1 π2)
-            (aux : Aux Reduction Γ t1 π1 t2 π2 h2)
-    : ConversionResult (conv_term leq Γ t1 π1 t2 π2). Admitted.
-  Axiom unfold_one_fix : forall (Γ : context) (mfix : mfixpoint term)
-            (idx : nat) (π : stack) (h : wtp Γ (tFix mfix idx) π),
-    option (term * stack).
-
-  Derive NoConfusion NoConfusionHom for option.
-
-  Lemma unfold_one_fix_red_zipp :
-    forall Γ mfix idx π h fn ξ,
-      Some (fn, ξ) = unfold_one_fix Γ mfix idx π h ->
-      forall Σ (wfΣ : abstract_env_ext_rel X Σ), ∥ red (fst Σ) (Γ ,,, stack_context π) (zipp (tFix mfix idx) π) (zipp fn ξ) ∥.
-Admitted.
-
-  Lemma unfold_one_fix_red_zippx :
-    forall Γ mfix idx π h fn ξ,
-      Some (fn, ξ) = unfold_one_fix Γ mfix idx π h ->
-      forall Σ (wfΣ : abstract_env_ext_rel X Σ), ∥ red (fst Σ) Γ (zippx (tFix mfix idx) π) (zippx fn ξ) ∥.
-Admitted.
-
-  Lemma unfold_one_fix_red :
-    forall Γ mfix idx π h fn ξ,
-      Some (fn, ξ) = unfold_one_fix Γ mfix idx π h ->
-      forall Σ (wfΣ : abstract_env_ext_rel X Σ), ∥ red (fst Σ) Γ (zipc (tFix mfix idx) π) (zipc fn ξ) ∥.
-Admitted.
-
-  Lemma unfold_one_fix_cored :
-    forall Γ mfix idx π h fn ξ,
-      Some (fn, ξ) = unfold_one_fix Γ mfix idx π h ->
-      forall Σ (wfΣ : abstract_env_ext_rel X Σ), cored (fst Σ) Γ (zipc fn ξ) (zipc (tFix mfix idx) π).
-Admitted.
-
-  Lemma unfold_one_fix_decompose :
-    forall Γ mfix idx π h fn ξ,
-      Some (fn, ξ) = unfold_one_fix Γ mfix idx π h ->
-      snd (decompose_stack π) = snd (decompose_stack ξ).
-Admitted.
-
-  Lemma unfold_one_fix_None Γ mfix idx π wf :
-    None = unfold_one_fix Γ mfix idx π wf ->
-    ∥∑args,
-     forall Σ (wfΣ : abstract_env_ext_rel X Σ),
-      All2 (red Σ (Γ,,, stack_context π)) (decompose_stack π).1 args ×
-      whnf RedFlags.default Σ (Γ,,, stack_context π) (mkApps (tFix mfix idx) args)∥.
-Admitted.
-
-  Inductive prog_view : term -> term -> Type :=
-  | prog_view_App u1 v1 u2 v2 :
-      prog_view (tApp u1 v1) (tApp u2 v2)
-
-  | prog_view_Const c1 u1 c2 u2 :
-      prog_view (tConst c1 u1) (tConst c2 u2)
-
-  | prog_view_Lambda na1 A1 b1 na2 A2 b2 :
-      prog_view (tLambda na1 A1 b1) (tLambda na2 A2 b2)
-
-  | prog_view_Prod na1 A1 B1 na2 A2 B2 :
-      prog_view (tProd na1 A1 B1) (tProd na2 A2 B2)
-
-  | prog_view_Case ci p c brs ci' p' c' brs' :
-      prog_view (tCase ci p c brs) (tCase ci' p' c' brs')
-
-  | prog_view_Proj p c p' c' :
-      prog_view (tProj p c) (tProj p' c')
-
-  | prog_view_Fix mfix idx mfix' idx' :
-      prog_view (tFix mfix idx) (tFix mfix' idx')
-
-  | prog_view_CoFix mfix idx mfix' idx' :
-      prog_view (tCoFix mfix idx) (tCoFix mfix' idx')
-
-  | prog_view_other :
-      forall u v, prog_discr u v -> prog_view u v.
-
-  Lemma prog_viewc u v : prog_view u v.
-    Admitted.
-
-  Lemma welltyped_wf_local Σ Γ t :
-    welltyped Σ Γ t ->
-    ∥ wf_local Σ Γ ∥.
-Admitted.
-
-  Definition eqb_universe_instance_gen eq u v :=
-    forallb2 eq (map Universe.make u) (map Universe.make v).
-
-  Definition eqb_universe_instance :=
-    eqb_universe_instance_gen (abstract_env_eq X).
-
-  Lemma eqb_universe_instance_spec :
-    forall u v Σ (wfΣ : abstract_env_ext_rel X Σ),
-      forallb (wf_universeb Σ) (map Universe.make u) ->
-      forallb (wf_universeb Σ) (map Universe.make v) ->
-      eqb_universe_instance u v ->
-      R_universe_instance (eq_universe (global_ext_constraints Σ)) u v.
-Admitted.
-
-  Arguments LevelSet.mem : simpl never.
-
-  Definition abstract_conv_pb_relb `{cf : checker_flags}
-    (pb : conv_pb) :=
-    match pb with
-    | Conv => abstract_env_eq X
-    | Cumul => abstract_env_leq X
-    end.
-
-  Lemma compare_universeb_complete Σ (wfΣ : abstract_env_ext_rel X Σ) leq u u' :
-    wf_universe Σ u ->
-    wf_universe Σ u' ->
-    compare_universe leq (global_ext_constraints Σ) u u' ->
-    abstract_conv_pb_relb leq u u'.
-Admitted.
-
-  Lemma get_level_make l :
-    LevelExpr.get_level (LevelExpr.make l) = l.
-Admitted.
-
-  Lemma compare_universeb_make_complete Σ (wfΣ : abstract_env_ext_rel X Σ) leq x y :
-    wf_universe_level Σ x ->
-    wf_universe_level Σ y ->
-    compare_universe leq (global_ext_constraints Σ) (Universe.make x) (Universe.make y) ->
-    abstract_conv_pb_relb leq (Universe.make x) (Universe.make y).
-Admitted.
-
-  Lemma eqb_universe_instance_complete Σ (wfΣ : abstract_env_ext_rel X Σ) u u' :
-    wf_universe_instance Σ u ->
-    wf_universe_instance Σ u' ->
-    R_universe_instance (eq_universe (global_ext_constraints Σ)) u u' ->
-    eqb_universe_instance u u'.
-Admitted.
-
-  Lemma compare_universe_variance_complete Σ (wfΣ : abstract_env_ext_rel X Σ) leq v u u' :
-    wf_universe_level Σ u ->
-    wf_universe_level Σ u' ->
-    R_universe_variance (eq_universe Σ) (compare_universe leq Σ) v u u' ->
-    compare_universe_variance (abstract_env_eq X) (abstract_conv_pb_relb leq) v u u'.
-Admitted.
-
-  Lemma compare_universe_instance_variance_complete Σ (wfΣ : abstract_env_ext_rel X Σ) leq v u u' :
-    wf_universe_instance Σ u ->
-    wf_universe_instance Σ u' ->
-    R_universe_instance_variance (eq_universe Σ) (compare_universe leq Σ) v u u' ->
-    compare_universe_instance_variance (abstract_env_eq X) (abstract_conv_pb_relb leq) v u u'.
-Admitted.
-
-  Lemma consistent_instance_ext_wf Σ udecl u :
-    consistent_instance_ext Σ udecl u ->
-    wf_universe_instance Σ u.
-Admitted.
-
-  Lemma welltyped_zipc_tConst_inv Σ (wfΣ : abstract_env_ext_rel X Σ) Γ c u π :
-    welltyped Σ Γ (zipc (tConst c u) π) ->
-    exists cst,
-      declared_constant Σ c cst
-      × consistent_instance_ext Σ (cst_universes cst) u.
-Admitted.
-
-  Lemma red_conv_cum_l {leq Γ u v Σ}{wfΣ : abstract_env_ext_rel X Σ} :
-    Σ ;;; Γ ⊢ u ⇝ v -> conv_cum leq Σ Γ u v.
-Admitted.
-
-  Lemma red_conv_cum_r {leq Γ u v Σ}{wfΣ : abstract_env_ext_rel X Σ} :
-    Σ ;;; Γ ⊢ u ⇝ v -> conv_cum leq Σ Γ v u.
-Admitted.
-
-  Lemma closed_red_zipp {Σ Γ t u π} :
-    is_open_term Γ (zipp t π) ->
-    Σ ;;; Γ ⊢ t ⇝ u ->
-    Σ ;;; Γ ⊢ zipp t π ⇝ zipp u π.
-Admitted.
-
-  Ltac specialize_Σ wfΣ :=
-    repeat match goal with | h : _ |- _ => specialize (h _ wfΣ) end.
-
-  Lemma unfold_constants (Γ : context) (leq : conv_pb)
-            (c : kername) (u : Instance.t) (π1 : stack)
-            (h1 : wtp Γ (tConst c u) π1)
-            (c' : kername) (u' : Instance.t) (π2 : stack)
-            (h2 : wtp Γ (tConst c' u') π2)
-            (ne : c <> c' \/ (c = c' /\ ~eqb_universe_instance u u'))
-            (hx : conv_stack_ctx Γ π1 π2)
-            (aux : Aux Term Γ (tConst c u) π1 (tConst c' u') π2 h2)
-    : ConversionResult (conv_term leq Γ (tConst c u) π1 (tConst c' u') π2).
-    Admitted.
-
-  Lemma welltyped_zipc_tCase_brs_length Σ (wfΣ : abstract_env_ext_rel X Σ) Γ ci motive discr brs π :
-    welltyped Σ Γ (zipc (tCase ci motive discr brs) π) ->
-    exists mib oib, declared_inductive Σ ci mib oib /\ #|brs| = #|ind_ctors oib|.
-Admitted.
-
-  Lemma isconv_context_aux
-            (Γ Γ' Δ Δ' : context)
-            (cc : forall Σ (wfΣ : abstract_env_ext_rel X Σ), ∥Σ ⊢ Γ = Γ'∥)
-            (check :
-               forall (leq : conv_pb) (Δh : context_hole) (t : term) (Δh' : context_hole) (t' : term),
-                 Δ = fill_context_hole Δh t ->
-                 Δ' = fill_context_hole Δh' t' ->
-                 (forall Σ (wfΣ : abstract_env_ext_rel X Σ), ∥ ws_cumul_ctx_pb_rel Conv Σ Γ (context_hole_context Δh) (context_hole_context Δh')∥) ->
-                 ConversionResult (forall Σ (wfΣ : abstract_env_ext_rel X Σ), conv_cum leq Σ (Γ,,, context_hole_context Δh) t t'))
-            (Δpre Δ'pre Δpost Δ'post : context)
-            (eq : Δ = Δpre ,,, Δpost)
-            (eq' : Δ' = Δ'pre ,,, Δ'post) :
-    ConversionResult (forall Σ (wfΣ : abstract_env_ext_rel X Σ), ∥ws_cumul_ctx_pb_rel Conv Σ Γ Δpre Δ'pre∥).
-  Admitted.
-
-  Definition isconv_context
-            (Γ Γ' Δ Δ' : context)
-            (cc : forall Σ (wfΣ : abstract_env_ext_rel X Σ), ∥ Σ ⊢ Γ = Γ' ∥)
-            (check :
-               forall (leq : conv_pb) (Δh : context_hole) (t : term) (Δh' : context_hole) (t' : term),
-                 Δ = fill_context_hole Δh t ->
-                 Δ' = fill_context_hole Δh' t' ->
-                 (forall Σ (wfΣ : abstract_env_ext_rel X Σ),  ∥ws_cumul_ctx_pb_rel Conv Σ Γ (context_hole_context Δh) (context_hole_context Δh')∥) ->
-                 ConversionResult (forall Σ (wfΣ : abstract_env_ext_rel X Σ), conv_cum leq Σ (Γ,,, context_hole_context Δh) t t'))
-    : ConversionResult (forall Σ (wfΣ : abstract_env_ext_rel X Σ), ∥ws_cumul_ctx_pb_rel Conv Σ Γ Δ Δ'∥) :=
-    isconv_context_aux Γ Γ' Δ Δ' cc check Δ Δ' [] [] eq_refl eq_refl.
-
-  Lemma case_conv_brs_inv {Γ ci br br' p c brs1 brs2 π}
-  (h : wtp Γ (tCase ci p c (brs1 ++ br :: brs2)) π)
-  (p' : predicate term) (c' : term) (brs1' brs2' : list (branch term))
-  (π' : stack) (h' : wtp Γ (tCase ci p' c' (brs1' ++ br' :: brs2')) π')
-  (hx : conv_stack_ctx Γ π π')
-  (hp : forall Σ (wfΣ : abstract_env_ext_rel X Σ), ∥ ws_cumul_pb_predicate Σ (Γ ,,, stack_context π) p p' ∥)
-  (h1 : forall Σ (wfΣ : abstract_env_ext_rel X Σ), ∥ ws_cumul_pb_brs Σ (Γ ,,, stack_context π) p brs1 brs1' ∥) :
-  ∥ ∑ mdecl idecl,
-    [× forall Σ (wfΣ : abstract_env_ext_rel X Σ), declared_inductive Σ ci mdecl idecl,
-       #|pparams p| = ind_npars mdecl,
-       #|pparams p'| = ind_npars mdecl,
-       eq_context_gen eq eq br.(bcontext) br'.(bcontext),
-       test_context_k (fun k : nat => on_free_vars (closedP k (fun _ : nat => true)))
-         #|pparams p| br.(bcontext) &
-       test_context_k (fun k : nat => on_free_vars (closedP k (fun _ : nat => true)))
-         #|pparams p'| br'.(bcontext)] ∥.
-Admitted.
-
-  Lemma isconv_branches (Γ : context)
-    (ci : case_info)
-    (p : predicate term) (c : term) (brs1 brs2 : list (branch term))
-    (π : stack) (h : wtp Γ (tCase ci p c (brs1 ++ brs2)) π)
-    (p' : predicate term) (c' : term) (brs1' brs2' : list (branch term))
-    (π' : stack) (h' : wtp Γ (tCase ci p' c' (brs1' ++ brs2')) π')
-    (hx : conv_stack_ctx Γ π π')
-    (hp : forall Σ (wfΣ : abstract_env_ext_rel X Σ), ∥ ws_cumul_pb_predicate Σ (Γ ,,, stack_context π) p p' ∥)
-    (h1 : forall Σ (wfΣ : abstract_env_ext_rel X Σ), ∥ ws_cumul_pb_brs Σ (Γ ,,, stack_context π) p brs1 brs1' ∥)
-    (aux : Aux Term Γ (tCase ci p c (brs1 ++ brs2)) π (tCase ci p' c' (brs1' ++ brs2')) π' h')
-    : ConversionResult (forall Σ (wfΣ : abstract_env_ext_rel X Σ), ∥ ws_cumul_pb_brs Σ (Γ ,,, stack_context π) p brs2 brs2' ∥).
-
-    Admitted.
-
-  Lemma isconv_branches' (Γ : context)
-    (ci : case_info)
-    (p : predicate term) (c : term) (brs : list (branch term))
-    (π : stack) (h : wtp Γ (tCase ci p c brs) π)
-    (ci' : case_info)
-    (p' : predicate term) (c' : term) (brs' : list (branch term))
-    (π' : stack) (h' : wtp Γ (tCase ci' p' c' brs') π')
-    (hx : conv_stack_ctx Γ π π')
-    (hp : forall Σ (wfΣ : abstract_env_ext_rel X Σ), ∥ ws_cumul_pb_predicate Σ (Γ ,,, stack_context π) p p' ∥)
-    (ei : ci = ci')
-    (aux : Aux Term Γ (tCase ci p c brs) π (tCase ci' p' c' brs') π' h')
-    : ConversionResult (forall Σ (wfΣ : abstract_env_ext_rel X Σ), ∥ ws_cumul_pb_brs Σ (Γ ,,, stack_context π) p brs brs' ∥).
-Admitted.
-
 
   Inductive fix_kind :=
   | IndFix
@@ -972,50 +1166,6 @@ Admitted.
     | IndFix => Fix
     | CoIndFix => CoFix
     end.
-
-  Definition mFixRargMismatch fk :=
-    match fk with
-    | IndFix => FixRargMismatch
-    | CoIndFix => CoFixRargMismatch
-    end.
-
-  Definition mFixMfixMismatch fk :=
-    match fk with
-    | IndFix => FixMfixMismatch
-    | CoIndFix => CoFixMfixMismatch
-    end.
-
-  Lemma isws_cumul_pb_fix_types (fk : fix_kind) (Γ : context)
-    (idx : nat)
-    (mfix1 mfix2 : mfixpoint term) (π : stack)
-    (h : wtp Γ (mFix fk (mfix1 ++ mfix2) idx) π)
-    (mfix1' mfix2' : mfixpoint term) (π' : stack)
-    (h' : wtp Γ (mFix fk (mfix1' ++ mfix2') idx) π')
-    (hx : conv_stack_ctx Γ π π')
-    (h1 : ∥ All2 (fun u v =>
-                   (forall Σ (wfΣ : abstract_env_ext_rel X Σ), Σ ;;; Γ ,,, stack_context π ⊢ u.(dtype) = v.(dtype)) ×
-                   (u.(rarg) = v.(rarg)) * eq_binder_annot u.(dname) v.(dname)
-            ) mfix1 mfix1' ∥)
-    (aux : Aux Term Γ (mFix fk (mfix1 ++ mfix2) idx) π (mFix fk (mfix1' ++ mfix2') idx) π' h')
-    : ConversionResult (∥ All2 (fun u v =>
-          (forall Σ (wfΣ : abstract_env_ext_rel X Σ), Σ ;;; Γ ,,, stack_context π ⊢ u.(dtype) = v.(dtype)) ×
-          (u.(rarg) = v.(rarg)) * eq_binder_annot u.(dname) v.(dname)
-                          ) mfix2 mfix2' ∥).
-    Admitted.
-
-  Lemma conv_context_decl Pcmp :
-    forall Σ Γ Δ d d',
-      conv_context Pcmp Σ Γ Δ ->
-      conv_decls Pcmp Σ Γ Δ d d' ->
-      conv_context Pcmp Σ (Γ ,, d) (Δ ,, d').
-Admitted.
-
-  Lemma stack_entry_context_mFix_mfix_bd :
-    forall fk na ty ra mfix1 mfix2 idx,
-      stack_entry_context (mFix_mfix fk (mfix1, def_hole_body na ty ra, mfix2) idx) =
-      fix_context_alt (map def_sig mfix1 ++ (na,ty) :: map def_sig mfix2).
-admit.
-Defined.
 
   Equations isws_cumul_pb_fix_bodies (fk : fix_kind) (Γ : context) (idx : nat)
     (mfix1 mfix2 : mfixpoint term) (π : stack)
@@ -1099,3 +1249,4 @@ admit.
   Next Obligation.
 admit.
 Defined.
+
